acorn-examples/Sorter.v
@@ -36,55 +36,59 @@ Local Open Scope vector_scope.
 Section WithCava.
   Context {signal} `{Cava signal} `{Monad cava}.
 
-Definition twoSorter {signal} `{Cava signal} `{Monad cava} {n}
-                     (ab:  signal (Vec (Vec Bit n) 2)) :
-                     cava (signal (Vec (Vec Bit n) 2)) :=
-   let a := indexConst ab 0 in
-   let b := indexConst ab 1 in
-   comparison <- greaterThanOrEqual a b ;;
-   negComparison <- inv comparison ;;
-   let sorted : Vector.t (signal (Vec Bit n)) 2 :=
-     [indexAt ab (unpeel [comparison]);
-      indexAt ab (unpeel [negComparison])] in
-   ret (unpeel sorted).
+  Definition twoSorter {signal} `{Cava signal} `{Monad cava} {n}
+                      (ab:  signal (Vec (Vec Bit n) 2)) :
+                      cava (signal (Vec (Vec Bit n) 2)) :=
+    let a := indexConst ab 0 in
+    let b := indexConst ab 1 in
+    comparison <- greaterThanOrEqual a b ;;
+    negComparison <- inv comparison ;;
+    let sorted : Vector.t (signal (Vec Bit n)) 2 :=
+      [indexAt ab (unpeel [comparison]);
+        indexAt ab (unpeel [negComparison])] in
+    ret (unpeel sorted).
+
+  End WithCava.
+
+  Definition two_sorter_Interface bitSize
+    := combinationalInterface "two_sorter"
+      [mkPort "inputs" (Vec (Vec Bit bitSize) 2)]
+      [mkPort "sorted" (Vec (Vec Bit bitSize) 2)]
+      [].
+
+  Definition two_sorter_Netlist
+    := makeNetlist (two_sorter_Interface 8) twoSorter.
+
+  Definition v0 := N2Bv_sized 8   5.
+  Definition v1 := N2Bv_sized 8 157.
+  Definition v2 := N2Bv_sized 8 255.
+  Definition v3 := N2Bv_sized 8  63.
+
+  Definition two_sorter_tb_inputs : list (Vector.t (Bvector 8) _) :=
+    [[v0; v1];
+    [v1; v0];
+    [v1; v2];
+    [v2; v1];
+    [v2; v3];
+    [v3; v2]
+    ].
+
+  Definition adder_tree4_8_tb_expected_outputs : list (Vector.t (Bvector 8) _) :=
+    map (fun i => combinational (twoSorter i)) two_sorter_tb_inputs.
+
+  Definition two_sorter_tb :=
+    testBench "two_sorter_tb" (two_sorter_Interface 8)
+    two_sorter_tb_inputs adder_tree4_8_tb_expected_outputs.
+
+  Definition twoSorterSpec {bw: nat} (ab : Vector.t (Bvector bw) 2) :
+                                    Vector.t (Bvector bw) 2 :=
+    let a := @Vector.nth_order _ 2 ab 0 (ltac:(lia)) in
+    let b := @Vector.nth_order _ 2 ab 1 (ltac:(lia)) in
+    if N.to_nat (Bv2N b) <=? N.to_nat (Bv2N a) then
+      [b; a]
+    else
+      [a; b].
+
+
 
 End WithCava.
-
-Definition two_sorter_Interface bitSize
-  := combinationalInterface "two_sorter"
-     [mkPort "inputs" (Vec (Vec Bit bitSize) 2)]
-     [mkPort "sorted" (Vec (Vec Bit bitSize) 2)]
-     [].
-
-Definition two_sorter_Netlist
-  := makeNetlist (two_sorter_Interface 8) twoSorter.
-
-Definition v0 := N2Bv_sized 8   5.
-Definition v1 := N2Bv_sized 8 157.
-Definition v2 := N2Bv_sized 8 255.
-Definition v3 := N2Bv_sized 8  63.
-
-Definition two_sorter_tb_inputs : list (Vector.t (Bvector 8) _) :=
-  [[v0; v1];
-   [v1; v0];
-   [v1; v2];
-   [v2; v1];
-   [v2; v3];
-   [v3; v2]
-  ].
-
-Definition adder_tree4_8_tb_expected_outputs : list (Vector.t (Bvector 8) _) :=
-  map (fun i => combinational (twoSorter i)) two_sorter_tb_inputs.
-
-Definition two_sorter_tb :=
-  testBench "two_sorter_tb" (two_sorter_Interface 8)
-  two_sorter_tb_inputs adder_tree4_8_tb_expected_outputs.
-
-Definition twoSorterSpec {bw: nat} (ab : Vector.t (Bvector bw) 2) :
-                                   Vector.t (Bvector bw) 2 :=
-  let a := @Vector.nth_order _ 2 ab 0 (ltac:(lia)) in
-  let b := @Vector.nth_order _ 2 ab 1 (ltac:(lia)) in
-  if N.to_nat (Bv2N b) <=? N.to_nat (Bv2N a) then
-    [b; a]
-  else
-    [a; b].
